Splinter/Paged/Bundle.i.dfy
@@ -6,9 +6,10 @@ include "../../Spec/RefinementObligation.s.dfy"
 // Hey look, this abstract journal satisfies the refinement.
 module AbstractJournalRefinement refines CoordinationSystemRefinement(AbstractJournal, AbstractMap) { }
 
-module ConcreteRefinementProof refines ImplementationObligation(AbstractJournalRefinement, AbstractMap) { }
+// can't get functors to do their thing. See branch splinter-jonh-modulefight
+//module ConcreteRefinementProof refines ImplementationObligation(AbstractJournalRefinement, AbstractMap) { }
 
-module ImplementationObligation(implementation: StateMachineIfc) refines RefinesIfc(implementation, CrashTolerantMapSpecMod) { }
+//module ImplementationObligation(implementation: StateMachineIfc) refines RefinesIfc(implementation, CrashTolerantMapSpecMod) { }
 
 // Ooh, and so does this Paged journal
 module PagedJournalRefinement refines CoordinationSystemRefinement(PagedJournal, AbstractMap) { }
